\band{0.0}{u} &=& \band{0.1}{u} - 0.3816 - 0.3159 \left[ \band{0.1}{(u-g)} - 1.3194 \right] \quad \mathrm{;}  \quad \sigma\left[\band{0.1}{(u-g)}\right] = 0.33\cr
\band{0.0}{g} &=& \band{0.1}{g} - 0.4075 - 0.4157 \left[ \band{0.1}{(g-r)} - 0.9688 \right] \quad \mathrm{;}  \quad \sigma\left[\band{0.1}{(g-r)}\right] = 0.24\cr
\band{0.0}{r} &=& \band{0.1}{r} - 0.2217 - 0.3943 \left[ \band{0.1}{(r-i)} - 0.4084 \right] \quad \mathrm{;}  \quad \sigma\left[\band{0.1}{(r-i)}\right] = 0.05\cr
\band{0.0}{i} &=& \band{0.1}{i} - 0.1932 - 0.6077 \left[ \band{0.1}{(i-z)} - 0.3397 \right] \quad \mathrm{;}  \quad \sigma\left[\band{0.1}{(i-z)}\right] = 0.10\cr
\band{0.0}{z} &=& \band{0.1}{z} - 0.1061 - 0.2356 \left[ \band{0.1}{(i-z)} - 0.3406 \right] \quad \mathrm{;}  \quad \sigma\left[\band{0.1}{(i-z)}\right] = 0.09\cr
\band{0.0}{z} &=& \band{0.1}{z} - 0.1269 - 0.3417 \left[ \band{0.1}{(z-J)} - 0.4595 \right] \quad \mathrm{;}  \quad \sigma\left[\band{0.1}{(z-J)}\right] = 0.18\cr
\band{0.0}{J} &=& \band{0.1}{J} - 0.1206 - 0.4732 \left[ \band{0.1}{(J-H)} - 0.2238 \right] \quad \mathrm{;}  \quad \sigma\left[\band{0.1}{(J-H)}\right] = 0.03\cr
\band{0.0}{H} &=& \band{0.1}{H} - 0.1337 - 0.1533 \left[ \band{0.1}{(H-K_s)} + 0.0174 \right] \quad \mathrm{;}  \quad \sigma\left[\band{0.1}{(H-K_s)}\right] = 0.02\cr
\band{0.0}{K_s} &=& \band{0.1}{K_s} - 0.0303 + 1.2333 \left[ \band{0.1}{(H-K_s)} + 0.0174 \right] \quad \mathrm{;}  \quad \sigma\left[\band{0.1}{(H-K_s)}\right] = 0.02\cr
\band{0.1}{u} &=& \band{0.0}{u} + 0.3891 + 0.3291 \left[ \band{0.0}{(u-g)} - 1.2458 \right] \quad \mathrm{;}  \quad \sigma\left[\band{0.0}{(u-g)}\right] = 0.35\cr
\band{0.1}{g} &=& \band{0.0}{g} + 0.3009 + 0.2725 \left[ \band{0.0}{(u-g)} - 1.2665 \right] \quad \mathrm{;}  \quad \sigma\left[\band{0.0}{(u-g)}\right] = 0.35\cr
\band{0.1}{g} &=& \band{0.0}{g} + 0.4015 + 0.6098 \left[ \band{0.0}{(g-r)} - 0.7778 \right] \quad \mathrm{;}  \quad \sigma\left[\band{0.0}{(g-r)}\right] = 0.17\cr
\band{0.1}{r} &=& \band{0.0}{r} + 0.2247 + 0.1388 \left[ \band{0.0}{(g-r)} - 0.7778 \right] \quad \mathrm{;}  \quad \sigma\left[\band{0.0}{(g-r)}\right] = 0.17\cr
\band{0.1}{i} &=& \band{0.0}{i} + 0.1961 + 0.6461 \left[ \band{0.0}{(r-i)} - 0.3841 \right] \quad \mathrm{;}  \quad \sigma\left[\band{0.0}{(r-i)}\right] = 0.08\cr
\band{0.1}{z} &=& \band{0.0}{z} + 0.1350 + 0.6294 \left[ \band{0.0}{(i-z)} - 0.2791 \right] \quad \mathrm{;}  \quad \sigma\left[\band{0.0}{(i-z)}\right] = 0.09\cr
\band{0.1}{J} &=& \band{0.0}{J} + 0.1121 + 0.0828 \left[ \band{0.0}{(z-J)} - 0.4389 \right] \quad \mathrm{;}  \quad \sigma\left[\band{0.0}{(z-J)}\right] = 0.14\cr
\band{0.1}{J} &=& \band{0.0}{J} + 0.1189 - 0.1139 \left[ \band{0.0}{(J-H)} - 0.2436 \right] \quad \mathrm{;}  \quad \sigma\left[\band{0.0}{(J-H)}\right] = 0.03\cr
\band{0.1}{H} &=& \band{0.0}{H} + 0.1336 + 0.1114 \left[ \band{0.0}{(J-H)} - 0.2437 \right] \quad \mathrm{;}  \quad \sigma\left[\band{0.0}{(J-H)}\right] = 0.03\cr
\band{0.1}{K_s} &=& \band{0.0}{K_s} + 0.0686 + 0.8895 \left[ \band{0.0}{(H-K_s)} + 0.1003 \right] \quad \mathrm{;}  \quad \sigma\left[\band{0.0}{(H-K_s)}\right] = 0.06\cr
\band{0.0}{U} &=& \band{0.1}{u} - 0.4570 - 0.3342 \left[ \band{0.1}{(u-g)} - 1.3211 \right] \quad \mathrm{;}  \quad \sigma\left[\band{0.1}{(u-g)}\right] = 0.33\cr
\band{0.0}{B} &=& \band{0.1}{g} - 0.1276 - 0.1009 \left[ \band{0.1}{(g-r)} - 0.9688 \right] \quad \mathrm{;}  \quad \sigma\left[\band{0.1}{(g-r)}\right] = 0.25\cr
\band{0.0}{V} &=& \band{0.1}{r} + 0.0633 + 0.0568 \left[ \band{0.1}{(g-r)} - 0.9688 \right] \quad \mathrm{;}  \quad \sigma\left[\band{0.1}{(g-r)}\right] = 0.24\cr
\band{0.0}{R_c} &=& \band{0.1}{i} + 0.0672 + 0.0781 \left[ \band{0.1}{(r-i)} - 0.4084 \right] \quad \mathrm{;}  \quad \sigma\left[\band{0.1}{(r-i)}\right] = 0.05\cr
\band{0.0}{I_c} &=& \band{0.1}{z} + 0.0135 + 0.0311 \left[ \band{0.1}{(i-z)} - 0.3397 \right] \quad \mathrm{;}  \quad \sigma\left[\band{0.1}{(i-z)}\right] = 0.09\cr
\band{0.0}{U} &=& \band{0.0}{u} - 0.0757 - 0.0189 \left[ \band{0.0}{(u-g)} - 1.2616 \right] \quad \mathrm{;}  \quad \sigma\left[\band{0.0}{(u-g)}\right] = 0.35\cr
\band{0.0}{B} &=& \band{0.0}{g} + 0.2747 + 0.4598 \left[ \band{0.0}{(g-r)} - 0.7778 \right] \quad \mathrm{;}  \quad \sigma\left[\band{0.0}{(g-r)}\right] = 0.17\cr
\band{0.0}{V} &=& \band{0.0}{r} + 0.2876 + 0.2246 \left[ \band{0.0}{(g-r)} - 0.7778 \right] \quad \mathrm{;}  \quad \sigma\left[\band{0.0}{(g-r)}\right] = 0.17\cr
\band{0.0}{R_c} &=& \band{0.0}{i} + 0.2640 + 0.6991 \left[ \band{0.0}{(r-i)} - 0.3846 \right] \quad \mathrm{;}  \quad \sigma\left[\band{0.0}{(r-i)}\right] = 0.08\cr
\band{0.0}{I_c} &=& \band{0.0}{z} + 0.1483 + 0.7035 \left[ \band{0.0}{(i-z)} - 0.2751 \right] \quad \mathrm{;}  \quad \sigma\left[\band{0.0}{(i-z)}\right] = 0.09\cr
\band{0.0}{u} &=& \band{0.0}{U} + 0.0771 + 0.0249 \left[ \band{0.0}{(U-B)} - 1.0511 \right] \quad \mathrm{;}  \quad \sigma\left[\band{0.0}{(U-B)}\right] = 0.28\cr
\band{0.0}{g} &=& \band{0.0}{B} - 0.2252 - 0.3709 \left[ \band{0.0}{(B-V)} - 0.6338 \right] \quad \mathrm{;}  \quad \sigma\left[\band{0.0}{(B-V)}\right] = 0.22\cr
\band{0.0}{r} &=& \band{0.0}{V} - 0.2640 - 0.1782 \left[ \band{0.0}{(B-V)} - 0.6327 \right] \quad \mathrm{;}  \quad \sigma\left[\band{0.0}{(B-V)}\right] = 0.22\cr
\band{0.0}{r} &=& \band{0.0}{V} - 0.2837 - 0.5431 \left[ \band{0.0}{(V-R)} - 0.4034 \right] \quad \mathrm{;}  \quad \sigma\left[\band{0.0}{(V-R)}\right] = 0.06\cr
\band{0.0}{i} &=& \band{0.0}{R_c} - 0.2287 - 0.6493 \left[ \band{0.0}{(R_c-I_c)} - 0.3445 \right] \quad \mathrm{;}  \quad \sigma\left[\band{0.0}{(R_c-I_c)}\right] = 0.13\cr
\band{0.0}{z} &=& \band{0.0}{I_c} - 0.0975 - 0.1322 \left[ \band{0.0}{(R_c-I_C)} - 0.3685 \right] \quad \mathrm{;}  \quad \sigma\left[\band{0.0}{(R_c-I_C)}\right] = 0.13\cr
