$u = \band{0.1}{u} - 0.3320 - 0.3050 \left[ (\band{0.1}{u}-\band{0.1}{g}) - 1.2863 \right] $ & $\sigma\left[\band{0.1}{u}-\band{0.1}{g}\right] = 0.27$ \cr
$g = \band{0.1}{g} - 0.3124 - 0.3483 \left[ (\band{0.1}{g}-\band{0.1}{r}) - 0.7221 \right] $ & $\sigma\left[\band{0.1}{g}-\band{0.1}{r}\right] = 0.20$ \cr
$r = \band{0.1}{r} - 0.2026 - 0.3731 \left[ (\band{0.1}{r}-\band{0.1}{i}) - 0.3532 \right] $ & $\sigma\left[\band{0.1}{r}-\band{0.1}{i}\right] = 0.06$ \cr
$i = \band{0.1}{i} - 0.1080 - 0.4266 \left[ (\band{0.1}{i}-\band{0.1}{z}) - 0.1917 \right] $ & $\sigma\left[\band{0.1}{i}-\band{0.1}{z}\right] = 0.13$ \cr
$z = \band{0.1}{i} - 0.3167 - 1.1993 \left[ (\band{0.1}{i}-\band{0.1}{z}) - 0.1917 \right] $ & $\sigma\left[\band{0.1}{i}-\band{0.1}{z}\right] = 0.13$ \cr
$u = U + 0.0682 + 0.0197 \left[ (U-B) - 0.9619 \right] $ & $\sigma\left[U-B\right] = 0.20$ \cr
$g = B - 0.2365 - 0.3373 \left[ (B-V) - 0.5900 \right] $ & $\sigma\left[B-V\right] = 0.17$ \cr
$r = V - 0.2586 - 0.4940 \left[ (V-R) - 0.3166 \right] $ & $\sigma\left[V-R\right] = 0.07$ \cr
$i = R - 0.2007 - 0.4213 \left[ (R-I) - 0.2653 \right] $ & $\sigma\left[R-I\right] = 0.12$ \cr
$z = R - 0.4093 - 1.2427 \left[ (R-I) - 0.2653 \right] $ & $\sigma\left[R-I\right] = 0.12$ \cr
$\band{0.1}{u} = U + 0.4000 + 0.4174 \left[ (U-B) - 0.9619 \right] $ & $\sigma\left[U-B\right] = 0.20$ \cr
$\band{0.1}{g} = U - 0.8860 - 0.9507 \left[ (U-B) - 0.9619 \right] $ & $\sigma\left[U-B\right] = 0.20$ \cr
$\band{0.1}{g} = B + 0.0760 + 0.0610 \left[ (B-V) - 0.5900 \right] $ & $\sigma\left[B-V\right] = 0.17$ \cr
$\band{0.1}{r} = B - 0.6461 - 1.0835 \left[ (B-V) - 0.5900 \right] $ & $\sigma\left[B-V\right] = 0.17$ \cr
$\band{0.1}{r} = V - 0.0560 - 0.1812 \left[ (V-R) - 0.3166 \right] $ & $\sigma\left[V-R\right] = 0.07$ \cr
$\band{0.1}{i} = R - 0.0927 + 0.0079 \left[ (R-I) - 0.2653 \right] $ & $\sigma\left[R-I\right] = 0.12$ \cr
$\band{0.1}{z} = R - 0.2842 - 1.0293 \left[ (R-I) - 0.2653 \right] $ & $\sigma\left[R-I\right] = 0.12$ \cr
$\band{0.1}{u} = u + 0.3320 + 0.3247 \left[ (u-g) - 1.2665 \right] $ & $\sigma\left[u-g\right] = 0.25$ \cr
$\band{0.1}{g} = u - 0.9543 - 0.7556 \left[ (u-g) - 1.2665 \right] $ & $\sigma\left[u-g\right] = 0.25$ \cr
$\band{0.1}{g} = g + 0.3126 + 0.4584 \left[ (g-r) - 0.6125 \right] $ & $\sigma\left[g-r\right] = 0.15$ \cr
$\band{0.1}{r} = g - 0.4096 - 0.8621 \left[ (g-r) - 0.6125 \right] $ & $\sigma\left[g-r\right] = 0.15$ \cr
$\band{0.1}{i} = r - 0.1507 - 0.3659 \left[ (r-i) - 0.2597 \right] $ & $\sigma\left[r-i\right] = 0.10$ \cr
$\band{0.1}{z} = i - 0.0832 - 0.7575 \left[ (i-z) - 0.2080 \right] $ & $\sigma\left[i-z\right] = 0.10$ \cr
$U = u - 0.0682 - 0.0139 \left[ (u-g) - 1.2665 \right] $ & $\sigma\left[u-g\right] = 0.25$ \cr
$B = u - 1.0303 - 0.7968 \left[ (u-g) - 1.2665 \right] $ & $\sigma\left[u-g\right] = 0.25$ \cr
$B = g + 0.2366 + 0.3888 \left[ (g-r) - 0.6125 \right] $ & $\sigma\left[g-r\right] = 0.15$ \cr
$V = g - 0.3535 - 0.7636 \left[ (g-r) - 0.6125 \right] $ & $\sigma\left[g-r\right] = 0.15$ \cr
$R = r - 0.0581 - 0.3771 \left[ (r-i) - 0.2597 \right] $ & $\sigma\left[r-i\right] = 0.10$ \cr
$I = i - 0.0643 - 0.7241 \left[ (i-z) - 0.2080 \right] $ & $\sigma\left[i-z\right] = 0.10$ \cr
$U = \band{0.1}{u} - 0.4002 - 0.3229 \left[ (\band{0.1}{u}-\band{0.1}{g}) - 1.2863 \right] $ & $\sigma\left[\band{0.1}{u}-\band{0.1}{g}\right] = 0.27$ \cr
$B = \band{0.1}{g} - 0.0760 - 0.0535 \left[ (\band{0.1}{g}-\band{0.1}{r}) - 0.7221 \right] $ & $\sigma\left[\band{0.1}{g}-\band{0.1}{r}\right] = 0.20$ \cr
$V = \band{0.1}{g} - 0.6660 - 0.9268 \left[ (\band{0.1}{g}-\band{0.1}{r}) - 0.7221 \right] $ & $\sigma\left[\band{0.1}{g}-\band{0.1}{r}\right] = 0.20$ \cr
$R = \band{0.1}{r} - 0.2606 - 0.9225 \left[ (\band{0.1}{r}-\band{0.1}{i}) - 0.3532 \right] $ & $\sigma\left[\band{0.1}{r}-\band{0.1}{i}\right] = 0.06$ \cr
$I = \band{0.1}{i} - 0.1727 - 0.9727 \left[ (\band{0.1}{i}-\band{0.1}{z}) - 0.1917 \right] $ & $\sigma\left[\band{0.1}{i}-\band{0.1}{z}\right] = 0.13$ \cr
